x86/proofs/bignum_triple_sm2_alt.ml
@@ -4,13 +4,13 @@
  *)
 
 (* ========================================================================= *)
-(* Tripling modulo p_256, the field characteristic for the NIST P-256 curve. *)
+(* Tripling modulo p_sm2, the field characteristic for the CC SM2 curve.     *)
 (* ========================================================================= *)
 
-(**** print_literal_from_elf "x86/p256/bignum_triple_p256_alt.o";;
+(**** print_literal_from_elf "x86/sm2/bignum_triple_sm2_alt.o";;
  ****)
 
-let bignum_triple_p256_alt_mc = define_assert_from_elf "bignum_triple_p256_alt_mc" "x86/p256/bignum_triple_p256_alt.o"
+let bignum_triple_sm2_alt_mc = define_assert_from_elf "bignum_triple_sm2_alt_mc" "x86/sm2/bignum_triple_sm2_alt.o"
 [
   0xb9; 0x03; 0x00; 0x00; 0x00;
                            (* MOV (% ecx) (Imm32 (word 3)) *)
@@ -31,63 +31,60 @@ let bignum_triple_p256_alt_mc = define_assert_from_elf "bignum_triple_p256_alt_m
   0x48; 0x8b; 0x46; 0x18;  (* MOV (% rax) (Memop Quadword (%% (rsi,24))) *)
   0x48; 0xf7; 0xe1;        (* MUL2 (% rdx,% rax) (% rcx) *)
   0x49; 0x01; 0xc3;        (* ADD (% r11) (% rax) *)
-  0xb9; 0x01; 0x00; 0x00; 0x00;
-                           (* MOV (% ecx) (Imm32 (word 1)) *)
-  0x48; 0x11; 0xd1;        (* ADC (% rcx) (% rdx) *)
-  0x48; 0xb8; 0x01; 0x00; 0x00; 0x00; 0xff; 0xff; 0xff; 0xff;
-                           (* MOV (% rax) (Imm64 (word 18446744069414584321)) *)
-  0x48; 0xf7; 0xe1;        (* MUL2 (% rdx,% rax) (% rcx) *)
-  0x48; 0x89; 0xce;        (* MOV (% rsi) (% rcx) *)
-  0x48; 0xc1; 0xe6; 0x20;  (* SHL (% rsi) (Imm8 (word 32)) *)
-  0x49; 0x01; 0xc8;        (* ADD (% r8) (% rcx) *)
-  0x48; 0x83; 0xde; 0x00;  (* SBB (% rsi) (Imm8 (word 0)) *)
-  0x49; 0x29; 0xf1;        (* SUB (% r9) (% rsi) *)
-  0x49; 0x83; 0xda; 0x00;  (* SBB (% r10) (Imm8 (word 0)) *)
-  0x49; 0x19; 0xc3;        (* SBB (% r11) (% rax) *)
-  0x48; 0x19; 0xd1;        (* SBB (% rcx) (% rdx) *)
-  0x48; 0xff; 0xc9;        (* DEC (% rcx) *)
-  0xb8; 0xff; 0xff; 0xff; 0xff;
-                           (* MOV (% eax) (Imm32 (word 4294967295)) *)
-  0x48; 0x21; 0xc8;        (* AND (% rax) (% rcx) *)
-  0x31; 0xd2;              (* XOR (% edx) (% edx) *)
-  0x48; 0x29; 0xc2;        (* SUB (% rdx) (% rax) *)
-  0x49; 0x01; 0xc8;        (* ADD (% r8) (% rcx) *)
+  0x48; 0x83; 0xd2; 0x01;  (* ADC (% rdx) (Imm8 (word 1)) *)
+  0x48; 0x89; 0xd0;        (* MOV (% rax) (% rdx) *)
+  0x48; 0xc1; 0xe0; 0x20;  (* SHL (% rax) (Imm8 (word 32)) *)
+  0x48; 0x89; 0xc1;        (* MOV (% rcx) (% rax) *)
+  0x48; 0x29; 0xd0;        (* SUB (% rax) (% rdx) *)
+  0x49; 0x01; 0xd0;        (* ADD (% r8) (% rdx) *)
+  0x49; 0x11; 0xc1;        (* ADC (% r9) (% rax) *)
+  0x49; 0x83; 0xd2; 0x00;  (* ADC (% r10) (Imm8 (word 0)) *)
+  0x49; 0x11; 0xcb;        (* ADC (% r11) (% rcx) *)
+  0x48; 0x19; 0xd2;        (* SBB (% rdx) (% rdx) *)
+  0x48; 0xf7; 0xd2;        (* NOT (% rdx) *)
+  0x48; 0xb8; 0x00; 0x00; 0x00; 0x00; 0xff; 0xff; 0xff; 0xff;
+                           (* MOV (% rax) (Imm64 (word 18446744069414584320)) *)
+  0x48; 0x21; 0xd0;        (* AND (% rax) (% rdx) *)
+  0x48; 0xb9; 0xff; 0xff; 0xff; 0xff; 0xfe; 0xff; 0xff; 0xff;
+                           (* MOV (% rcx) (Imm64 (word 18446744069414584319)) *)
+  0x48; 0x21; 0xd1;        (* AND (% rcx) (% rdx) *)
+  0x49; 0x01; 0xd0;        (* ADD (% r8) (% rdx) *)
   0x4c; 0x89; 0x07;        (* MOV (Memop Quadword (%% (rdi,0))) (% r8) *)
   0x49; 0x11; 0xc1;        (* ADC (% r9) (% rax) *)
   0x4c; 0x89; 0x4f; 0x08;  (* MOV (Memop Quadword (%% (rdi,8))) (% r9) *)
-  0x49; 0x83; 0xd2; 0x00;  (* ADC (% r10) (Imm8 (word 0)) *)
+  0x49; 0x11; 0xd2;        (* ADC (% r10) (% rdx) *)
   0x4c; 0x89; 0x57; 0x10;  (* MOV (Memop Quadword (%% (rdi,16))) (% r10) *)
-  0x49; 0x11; 0xd3;        (* ADC (% r11) (% rdx) *)
+  0x49; 0x11; 0xcb;        (* ADC (% r11) (% rcx) *)
   0x4c; 0x89; 0x5f; 0x18;  (* MOV (Memop Quadword (%% (rdi,24))) (% r11) *)
   0xc3                     (* RET *)
 ];;
 
-let BIGNUM_TRIPLE_P256_ALT_EXEC = X86_MK_CORE_EXEC_RULE bignum_triple_p256_alt_mc;;
+let BIGNUM_TRIPLE_SM2_ALT_EXEC = X86_MK_CORE_EXEC_RULE bignum_triple_sm2_alt_mc;;
 
 (* ------------------------------------------------------------------------- *)
 (* Proof.                                                                    *)
 (* ------------------------------------------------------------------------- *)
 
-let p_256 = new_definition `p_256 = 115792089210356248762697446949407573530086143415290314195533631308867097853951`;;
+let p_sm2 = new_definition `p_sm2 = 0xFFFFFFFEFFFFFFFFFFFFFFFFFFFFFFFFFFFFFFFF00000000FFFFFFFFFFFFFFFF`;;
 
-let p256genshortredlemma = prove
+let sm2genshortredlemma = prove
  (`!n. n < 3 * 2 EXP 256
        ==> let q = (n DIV 2 EXP 256) + 1 in
            q <= 3 /\
-           q * p_256 <= n + p_256 /\
-           n < q * p_256 + p_256`,
-  CONV_TAC(TOP_DEPTH_CONV let_CONV) THEN REWRITE_TAC[p_256] THEN ARITH_TAC);;
+           q * p_sm2 <= n + p_sm2 /\
+           n < q * p_sm2 + p_sm2`,
+  CONV_TAC(TOP_DEPTH_CONV let_CONV) THEN REWRITE_TAC[p_sm2] THEN ARITH_TAC);;
 
-let BIGNUM_TRIPLE_P256_ALT_CORRECT = time prove
+let BIGNUM_TRIPLE_SM2_ALT_CORRECT = time prove
  (`!z x n pc.
-        nonoverlapping (word pc,0x98) (z,8 * 4)
+        nonoverlapping (word pc,0x95) (z,8 * 4)
         ==> ensures x86
-             (\s. bytes_loaded s (word pc) (BUTLAST bignum_triple_p256_alt_mc) /\
+             (\s. bytes_loaded s (word pc) (BUTLAST bignum_triple_sm2_alt_mc) /\
                   read RIP s = word pc /\
                   C_ARGUMENTS [z; x] s /\
                   bignum_from_memory (x,4) s = n)
-             (\s. read RIP s = word (pc + 0x97) /\
-                  bignum_from_memory (z,4) s = (3 * n) MOD p_256)
+             (\s. read RIP s = word (pc + 0x94) /\
+                  bignum_from_memory (z,4) s = (3 * n) MOD p_sm2)
           (MAYCHANGE [RIP; RSI; RAX; RCX; RDX; R8; R9; R10; R11] ,,
            MAYCHANGE SOME_FLAGS ,,
            MAYCHANGE [memory :> bignum(z,4)])`,
@@ -101,10 +98,10 @@ let BIGNUM_TRIPLE_P256_ALT_CORRECT = time prove
 
   (*** Input load and initial multiplication by 3 ***)
 
-  X86_ACCSTEPS_TAC BIGNUM_TRIPLE_P256_ALT_EXEC (1--20) (1--20) THEN
+  X86_ACCSTEPS_TAC BIGNUM_TRIPLE_SM2_ALT_EXEC (1--19) (1--19) THEN
 
   SUBGOAL_THEN
-   `bignum_of_wordlist [mullo_s3; sum_s9; sum_s14; sum_s18; sum_s20] =
+   `bignum_of_wordlist [mullo_s3; sum_s9; sum_s14; sum_s18; sum_s19] =
     2 EXP 256 + 3 * n`
   ASSUME_TAC THENL
    [EXPAND_TAC "n" THEN
@@ -119,7 +116,7 @@ let BIGNUM_TRIPLE_P256_ALT_CORRECT = time prove
   SUBGOAL_THEN `h < 3` ASSUME_TAC THENL
    [UNDISCH_TAC `n < 2 EXP (64 * 4)` THEN EXPAND_TAC "h" THEN ARITH_TAC;
     ALL_TAC] THEN
-  SUBGOAL_THEN `sum_s20:int64 = word(h + 1)` SUBST_ALL_TAC THENL
+  SUBGOAL_THEN `sum_s19:int64 = word(h + 1)` SUBST_ALL_TAC THENL
    [EXPAND_TAC "h" THEN REWRITE_TAC[ARITH_RULE
      `(3 * n) DIV 2 EXP 256 + 1 = (2 EXP 256 + 3 * n) DIV 2 EXP 256`] THEN
     FIRST_X_ASSUM(fun th ->
@@ -127,86 +124,85 @@ let BIGNUM_TRIPLE_P256_ALT_CORRECT = time prove
     CONV_TAC(ONCE_DEPTH_CONV BIGNUM_OF_WORDLIST_DIV_CONV) THEN
     REWRITE_TAC[WORD_VAL];
     ALL_TAC] THEN
-  MP_TAC(SPEC `3 * n` p256genshortredlemma) THEN ASM_REWRITE_TAC[] THEN
+  MP_TAC(SPEC `3 * n` sm2genshortredlemma) THEN ASM_REWRITE_TAC[] THEN
   ANTS_TAC THENL
    [UNDISCH_TAC `n < 2 EXP (64 * 4)` THEN ARITH_TAC;
     CONV_TAC(LAND_CONV let_CONV) THEN STRIP_TAC] THEN
 
-  (*** Computation of 3 * n - (h + 1) * p_256 ***)
+  (*** Computation of 3 * n - (h + 1) * p_sm2 ***)
 
-  X86_ACCSTEPS_TAC BIGNUM_TRIPLE_P256_ALT_EXEC (25--31) (21--31) THEN
+  X86_ACCSTEPS_TAC BIGNUM_TRIPLE_SM2_ALT_EXEC (24--27) (20--29) THEN
   MP_TAC(SPECL
-   [`sum_s31:int64`;
-    `&(bignum_of_wordlist[sum_s25; sum_s27; sum_s28; sum_s29]):real`;
-    `256`; `3 * n`; `(h + 1) * p_256`]
+   [`word_neg(word(bitval(~carry_s27))):int64`;
+    `&(bignum_of_wordlist[sum_s24; sum_s25; sum_s26; sum_s27]):real`;
+    `256`; `3 * n`; `(h + 1) * p_sm2`]
    MASK_AND_VALUE_FROM_CARRY_LT) THEN
   ASM_REWRITE_TAC[] THEN ANTS_TAC THENL
-   [CONJ_TAC THENL
+   [REWRITE_TAC[GSYM WORD_NOT_MASK; REAL_VAL_WORD_NOT; DIMINDEX_64] THEN
+    CONJ_TAC THENL
      [MAP_EVERY UNDISCH_TAC
-       [`(h + 1) * p_256 <= 3 * n + p_256`;
-        `3 * n < (h + 1) * p_256 + p_256`] THEN
-      REWRITE_TAC[GSYM REAL_OF_NUM_CLAUSES; p_256] THEN REAL_ARITH_TAC;
+       [`(h + 1) * p_sm2 <= 3 * n + p_sm2`;
+        `3 * n < (h + 1) * p_sm2 + p_sm2`] THEN
+      REWRITE_TAC[GSYM REAL_OF_NUM_CLAUSES; p_sm2] THEN REAL_ARITH_TAC;
       ALL_TAC] THEN
     CONJ_TAC THENL
      [REWRITE_TAC[bignum_of_wordlist; GSYM REAL_OF_NUM_CLAUSES] THEN
       BOUNDER_TAC[];
       ALL_TAC] THEN
-
     SUBGOAL_THEN
      `&(3 * n):real =
-      &(bignum_of_wordlist [mullo_s3; sum_s9; sum_s14; sum_s18; word(h + 1)]) -
+      &(bignum_of_wordlist [mullo_s3; sum_s9; sum_s14; sum_s18; word (h + 1)]) -
       &2 pow 256`
     SUBST1_TAC THENL
      [ASM_REWRITE_TAC[GSYM REAL_OF_NUM_CLAUSES] THEN REAL_ARITH_TAC;
       ALL_TAC] THEN
-
-    REWRITE_TAC[p_256; bignum_of_wordlist; GSYM REAL_OF_NUM_CLAUSES] THEN
+    REWRITE_TAC[p_sm2; bignum_of_wordlist; GSYM REAL_OF_NUM_CLAUSES] THEN
     ACCUMULATOR_POP_ASSUM_LIST(MP_TAC o end_itlist CONJ) THEN
-    REWRITE_TAC[DIMINDEX_64] THEN UNDISCH_TAC `h < 3` THEN
+    UNDISCH_TAC `h < 3` THEN
     SPEC_TAC(`h:num`,`h:num`) THEN CONV_TAC EXPAND_CASES_CONV THEN
     CONV_TAC(DEPTH_CONV(NUM_RED_CONV ORELSEC WORD_RED_CONV ORELSEC
                         GEN_REWRITE_CONV I [BITVAL_CLAUSES])) THEN
-    REPEAT CONJ_TAC THEN
-    DISCH_THEN(fun th ->
-      (MP_TAC o end_itlist CONJ o DESUM_RULE o CONJUNCTS) th THEN
-      DISCH_THEN(fun th -> REWRITE_TAC[th]) THEN
-      CONV_TAC(RAND_CONV REAL_POLY_CONV) THEN
-      (MP_TAC o end_itlist CONJ o
-       filter (is_ratconst o rand o concl) o DECARRY_RULE o CONJUNCTS) th THEN
-      DISCH_THEN(fun th -> REWRITE_TAC[th]) THEN REAL_INTEGER_TAC);
+    REWRITE_TAC[REAL_VAL_WORD_MASK; DIMINDEX_64] THEN REPEAT CONJ_TAC THEN
+    DISCH_THEN(MP_TAC o end_itlist CONJ o DESUM_RULE o CONJUNCTS) THEN
+    DISCH_THEN(fun th -> REWRITE_TAC[th]) THEN REAL_INTEGER_TAC;
     ACCUMULATOR_POP_ASSUM_LIST(K ALL_TAC) THEN DISCARD_FLAGS_TAC THEN
+    REWRITE_TAC[WORD_ARITH `word_neg x = word_neg y <=> val x = val y`] THEN
+    REWRITE_TAC[VAL_WORD_BITVAL; EQ_BITVAL] THEN
+    REWRITE_TAC[TAUT `(~p <=> q) <=> (p <=> ~q)`] THEN
     DISCH_THEN(CONJUNCTS_THEN2 SUBST_ALL_TAC MP_TAC) THEN
+    RULE_ASSUM_TAC(REWRITE_RULE[COND_SWAP]) THEN
     REWRITE_TAC[MESON[REAL_MUL_RZERO; REAL_MUL_RID; REAL_ADD_RID; bitval]
      `(if p then x + a else x):real = x + a * &(bitval p)`] THEN
     DISCH_TAC] THEN
 
   (*** Final corrective masked addition ***)
 
-  X86_ACCSTEPS_TAC BIGNUM_TRIPLE_P256_ALT_EXEC [36;38;40;42] (32--43) THEN
+  X86_ACCSTEPS_TAC BIGNUM_TRIPLE_SM2_ALT_EXEC [34;36;38;40] (30--41) THEN
   ENSURES_FINAL_STATE_TAC THEN ASM_REWRITE_TAC[] THEN
+  RULE_ASSUM_TAC(REWRITE_RULE[WORD_NOT_MASK; NOT_LE]) THEN
   CONV_TAC(LAND_CONV BIGNUM_EXPAND_CONV) THEN ASM_REWRITE_TAC[] THEN
   CONV_TAC SYM_CONV THEN MATCH_MP_TAC MOD_UNIQ_BALANCED_REAL THEN
   MAP_EVERY EXISTS_TAC [`h + 1`; `256`] THEN
   ASM_REWRITE_TAC[] THEN
-  ABBREV_TAC `topcar <=> 3 * n < (h + 1) * p_256` THEN
+  ABBREV_TAC `topcar <=> 3 * n < (h + 1) * p_sm2` THEN
   FIRST_X_ASSUM(SUBST1_TAC o MATCH_MP (REAL_ARITH
    `x:real = &(3 * n) - y + z ==> &(3 * n) = x + y - z`)) THEN
-  REWRITE_TAC[p_256] THEN CONJ_TAC THENL [ARITH_TAC; ALL_TAC] THEN
+  REWRITE_TAC[p_sm2] THEN CONJ_TAC THENL [ARITH_TAC; ALL_TAC] THEN
   REWRITE_TAC[bignum_of_wordlist; GSYM REAL_OF_NUM_CLAUSES] THEN
   CONJ_TAC THENL [BOUNDER_TAC[]; ALL_TAC] THEN
-  REWRITE_TAC[GSYM REAL_OF_NUM_CLAUSES; p_256; bignum_of_wordlist] THEN
+  REWRITE_TAC[GSYM REAL_OF_NUM_CLAUSES; p_sm2; bignum_of_wordlist] THEN
   ACCUMULATOR_POP_ASSUM_LIST(MP_TAC o end_itlist CONJ o DESUM_RULE) THEN
   POP_ASSUM_LIST(K ALL_TAC) THEN
   BOOL_CASES_TAC `topcar:bool` THEN ASM_REWRITE_TAC[BITVAL_CLAUSES] THEN
   CONV_TAC WORD_REDUCE_CONV THEN
   DISCH_THEN(fun th -> REWRITE_TAC[th]) THEN REAL_INTEGER_TAC);;
 
-let BIGNUM_TRIPLE_P256_ALT_SUBROUTINE_CORRECT = time prove
+let BIGNUM_TRIPLE_SM2_ALT_SUBROUTINE_CORRECT = time prove
  (`!z x n pc stackpointer returnaddress.
-        nonoverlapping (word pc,0x98) (z,8 * 4) /\
+        nonoverlapping (word pc,0x95) (z,8 * 4) /\
         nonoverlapping (stackpointer,8) (z,8 * 4)
         ==> ensures x86
-             (\s. bytes_loaded s (word pc) bignum_triple_p256_alt_mc /\
+             (\s. bytes_loaded s (word pc) bignum_triple_sm2_alt_mc /\
                   read RIP s = word pc /\
                   read RSP s = stackpointer /\
                   read (memory :> bytes64 stackpointer) s = returnaddress /\
@@ -214,28 +210,28 @@ let BIGNUM_TRIPLE_P256_ALT_SUBROUTINE_CORRECT = time prove
                   bignum_from_memory (x,4) s = n)
              (\s. read RIP s = returnaddress /\
                   read RSP s = word_add stackpointer (word 8) /\
-                  bignum_from_memory (z,4) s = (3 * n) MOD p_256)
+                  bignum_from_memory (z,4) s = (3 * n) MOD p_sm2)
           (MAYCHANGE [RIP; RSP; RSI; RAX; RCX; RDX; R8; R9; R10; R11] ,,
            MAYCHANGE SOME_FLAGS ,,
            MAYCHANGE [memory :> bignum(z,4)])`,
-  X86_PROMOTE_RETURN_NOSTACK_TAC bignum_triple_p256_alt_mc
-      BIGNUM_TRIPLE_P256_ALT_CORRECT);;
+  X86_PROMOTE_RETURN_NOSTACK_TAC bignum_triple_sm2_alt_mc
+      BIGNUM_TRIPLE_SM2_ALT_CORRECT);;
 
 (* ------------------------------------------------------------------------- *)
 (* Correctness of Windows ABI version.                                       *)
 (* ------------------------------------------------------------------------- *)
 
-let windows_bignum_triple_p256_alt_mc = define_from_elf
-   "windows_bignum_triple_p256_alt_mc" "x86/p256/bignum_triple_p256_alt.obj";;
+let windows_bignum_triple_sm2_alt_mc = define_from_elf
+   "windows_bignum_triple_sm2_alt_mc" "x86/sm2/bignum_triple_sm2_alt.obj";;
 
-let WINDOWS_BIGNUM_TRIPLE_P256_ALT_SUBROUTINE_CORRECT = time prove
+let WINDOWS_BIGNUM_TRIPLE_SM2_ALT_SUBROUTINE_CORRECT = time prove
  (`!z x n pc stackpointer returnaddress.
         ALL (nonoverlapping (word_sub stackpointer (word 16),16))
-            [(word pc,0xa2); (x,8 * 4)] /\
-        nonoverlapping (word pc,0xa2) (z,8 * 4) /\
+            [(word pc,0x9f); (x,8 * 4)] /\
+        nonoverlapping (word pc,0x9f) (z,8 * 4) /\
         nonoverlapping (word_sub stackpointer (word 16),24) (z,8 * 4)
         ==> ensures x86
-             (\s. bytes_loaded s (word pc) windows_bignum_triple_p256_alt_mc /\
+             (\s. bytes_loaded s (word pc) windows_bignum_triple_sm2_alt_mc /\
                   read RIP s = word pc /\
                   read RSP s = stackpointer /\
                   read (memory :> bytes64 stackpointer) s = returnaddress /\
@@ -243,11 +239,11 @@ let WINDOWS_BIGNUM_TRIPLE_P256_ALT_SUBROUTINE_CORRECT = time prove
                   bignum_from_memory (x,4) s = n)
              (\s. read RIP s = returnaddress /\
                   read RSP s = word_add stackpointer (word 8) /\
-                  bignum_from_memory (z,4) s = (3 * n) MOD p_256)
+                  bignum_from_memory (z,4) s = (3 * n) MOD p_sm2)
           (MAYCHANGE [RIP; RSP; RAX; RCX; RDX; R8; R9; R10; R11] ,,
            MAYCHANGE SOME_FLAGS ,,
            MAYCHANGE [memory :> bignum(z,4);
                       memory :> bytes(word_sub stackpointer (word 16),16)])`,
   WINDOWS_X86_WRAP_NOSTACK_TAC
-    windows_bignum_triple_p256_alt_mc bignum_triple_p256_alt_mc
-    BIGNUM_TRIPLE_P256_ALT_CORRECT);;
+    windows_bignum_triple_sm2_alt_mc bignum_triple_sm2_alt_mc
+    BIGNUM_TRIPLE_SM2_ALT_CORRECT);;
